updating sk

clightplus/compiler/ClightPlusSkel.v
@@ -50,81 +50,245 @@ Definition gdef := globdef fundef type.
 
 Module GDef <: Typ. Definition t := gdef. End GDef.
 
-Module SkSort := AListSort GDef.
+Module SkGSort := AListSort GDef.
 
-Definition sort: alist gname gdef -> alist gname gdef := SkSort.sort.
+Definition gsort: alist gname gdef -> alist gname gdef := SkGSort.sort.
 
-Definition incl (sk0 sk1: alist gname gdef): Prop :=
-forall gn gd (IN: List.In (gn, gd) sk0),
-    List.In (gn, gd) sk1.
+Definition cdef := composite.
+
+Module CDef <: Typ. Definition t := cdef. End CDef.
+
+Module SkCSort := AIListSort CDef.
+
+Definition csort: alist positive cdef -> alist positive cdef := SkCSort.sort.
+
+Definition incl (sk0 sk1: (alist gname gdef) * (alist positive cdef)): Prop :=
+  (forall gn gd (IN: List.In (gn, gd) (fst sk0)), List.In (gn, gd) (fst sk1))
+  /\ (forall id co (IN: List.In (id, co) (snd sk0)), List.In (id, co) (snd sk1)).
+
+Definition struct_or_union_dec : forall x y: struct_or_union, {x = y} + {x <> y}.
+Proof.
+  i. destruct x, y.
+  - left. et.
+  - right. ss.
+  - right. ss.
+  - left. et.
+Defined.
+
+Definition members_dec : forall x y: members, {x = y} + {x <> y}.
+Proof.
+  i. revert y. induction x. 
+  - i. destruct y.
+    + left. et.
+    + right. ss.
+  - i. destruct y.
+    + right. ss.
+    + destruct a, p. destruct (dec i i0); cycle 1. { right. ii. apply n. clarify. }
+      subst. destruct (type_eq t t0); cycle 1. { right. ii. apply n. clarify. }
+      subst. destruct (IHx y). subst. left. et.
+      right. ii. apply n. clarify.
+Defined.
+
+Definition attr_dec : forall x y: attr, {x = y} + {x <> y}.
+Proof.
+  i. destruct x, y.
+  destruct attr_volatile; destruct attr_volatile0.
+  2,3: right; ii; clarify.
+  all: destruct attr_alignas; destruct attr_alignas0.
+  2,3,6,7: right; ii; clarify.
+  2,4: left; et.
+  all: destruct (N.eq_dec n n0); subst.
+  1,3: left; et.
+  all: right; ii; clarify.
+Defined.
+
+Definition composite_eq_dec : forall x y: composite, {x = y} + {x <> y}.
+Proof.
+  i. destruct x, y.
+  destruct (struct_or_union_dec co_su co_su0);
+  destruct (members_dec co_members co_members0);
+  destruct (attr_dec co_attr co_attr0);
+  destruct (Z.eq_dec co_sizeof co_sizeof0);
+  destruct (Z.eq_dec co_alignof co_alignof0);
+  destruct (Nat.eq_dec co_rank co_rank0).
+  { subst.
+    assert (co_sizeof_pos = co_sizeof_pos0) by apply proof_irr.
+    assert (co_alignof_two_p = co_alignof_two_p0) by apply proof_irr.
+    assert (co_sizeof_alignof = co_sizeof_alignof0) by apply proof_irr.
+    subst. left. et. }
+  all: right; ii; inv H; et.
+Defined.
+
+Definition check_compat_composite (l: alist ident composite) (cd: ident * composite) : bool :=
+  List.forallb
+    (fun cd' =>
+      if ident_eq (fst cd') (fst cd) then composite_eq_dec (snd cd) (snd cd') else true)
+    l.
+
+Definition filter_redefs (l1 l2: alist ident composite) :=
+  let names1 := map fst l1 in
+  List.filter (fun cd => negb (In_dec ident_eq (fst cd) names1)) l2.
+
+Definition _link_composite_defs (l1 l2: alist ident composite): option (alist ident composite) :=
+  if List.forallb (check_compat_composite l2) l1
+  then Some (l1 ++ filter_redefs l1 l2)
+  else None.
+
+Definition default_composite : composite.
+Proof.
+  econs.
+  - exact Struct.
+  - exact [].
+  - econs. { exact true. } { exact None. }
+  - exact 0.
+  - instantiate (1:=0%Z). nia.
+  - exists 0. ss.
+  - exists 0%Z. ss.
+Qed.
+
+Definition link_composite_defs (l1 l2: alist ident composite): alist ident composite :=
+  match _link_composite_defs l1 l2 with
+  | Some l => l
+  | None => [(xH, default_composite); (xH, default_composite)]
+  end.
+
+Definition add (sk0 sk1: (alist gname gdef) * (alist positive cdef)): (alist gname gdef) * (alist positive cdef) :=
+  let (g0, c0) := sk0 in
+  let (g1, c1) := sk1 in
+  (List.app g0 g1, link_composite_defs c0 c1).
+
+Definition sort (sk : (alist gname gdef) * (alist positive cdef)): (alist gname gdef) * (alist positive cdef) :=
+  let (g, c) := sk in
+  (gsort g, csort c).
+
+Definition wf (sk: (alist gname gdef) * (alist positive cdef)): Prop :=
+  let (g, c) := sk in
+  List.NoDup (List.map fst g) /\ List.NoDup (List.map fst c).
+
+Definition wf_dec (sk: (alist gname gdef) * (alist positive cdef)): {wf sk} + {~wf sk}.
+Proof.
+  destruct sk.
+  destruct (ListDec.NoDup_dec string_dec (map fst a));
+  destruct (ListDec.NoDup_dec Pos.eq_dec (map fst a0)).
+  - left. red. et.
+  - right. red. i. red in H. apply n0. des. et.
+  - right. red. i. red in H. apply n. des. et.
+  - right. red. i. red in H. apply n0. des. et.
+Defined.
 
 Program Definition gdefs: Sk.ld := 
-  @Sk.mk (alist gname gdef) nil (@List.app _) sort (fun sk => @List.NoDup _ (List.map fst sk)) (fun sk => ListDec.NoDup_dec string_dec (List.map fst sk)) incl
+  @Sk.mk ((alist gname gdef) * (alist positive cdef)) (nil, nil) add sort wf wf_dec incl
   _ _ _ _ _ _ _ _ _ _ _ _ _ _.
 Next Obligation.
   econs.
   - ii. ss.
-  - ii. eapply H0. eapply H. ss.
+  - ii. unfold incl in *. des. split.
+    + i. eapply H0. eapply H. ss.
+    + i. eapply H1. eapply H2. ss.
 Qed.
 Next Obligation.
-  ii. eapply Permutation.Permutation_in; [|apply IN].
-  eapply SkSort.sort_permutation.
+  split.
+  - ii. eapply Permutation.Permutation_in; [|apply IN].
+    eapply SkGSort.sort_permutation.
+  - ii. eapply Permutation.Permutation_in; [|apply IN].
+    eapply SkCSort.sort_permutation.
 Qed.
 Next Obligation.
-  ii. eapply Permutation.Permutation_in; [|apply IN].
-  symmetry. eapply SkSort.sort_permutation.
+  split.
+  - ii. eapply Permutation.Permutation_in; [|apply IN].
+    symmetry. eapply SkGSort.sort_permutation.
+  - ii. eapply Permutation.Permutation_in; [|apply IN].
+    symmetry. eapply SkCSort.sort_permutation.
 Qed.
 Next Obligation.
-  eapply SkSort.sort_add_comm. auto.
+  unfold sort, add, wf in *. des. f_equal.
+  - eapply SkGSort.sort_add_comm. auto.
+  - admit "sort_comm".
 Qed.
 Next Obligation.
-  eapply List.app_assoc.
+  unfold add. f_equal.
+  - eapply List.app_assoc.
+  - admit "assoc".
 Qed.
 Next Obligation.
-  rewrite List.app_nil_r. auto.
+  unfold link_composite_defs. ss. unfold filter_redefs. ss.
+  f_equal. induction a0; ss. f_equal. et.
 Qed.
 Next Obligation.
-  induction b; ss. red. i. ss. right. et.
+  unfold add. rewrite List.app_nil_r. f_equal.
+  unfold link_composite_defs. unfold _link_composite_defs. ss. unfold check_compat_composite.
+  ss. rewrite List.app_nil_r.
+  replace (if (forallb _ _) then _ else _) with (Some a0); et.
+  induction a0; ss. destruct forallb; ss.
 Qed.
 Next Obligation.
-  induction a; ss. red. i. ss. des; subst; et.
+  red. split; ss.
+  - induction a0; ss. i. ss. des; subst; et.
+  - admit "le_add".
 Qed.
 Next Obligation.
-  induction c; ss. red. i. ss. des; subst; et.
+  red. unfold add. ss. split; ss.
+  - induction a; ss. i. ss. des; subst; et.
+  - admit "le_add".
 Qed.
 Next Obligation.
-  eapply Permutation.Permutation_NoDup; [|et].
-  eapply Permutation.Permutation_map.
-  apply Permutation.Permutation_app_comm.
+  red. unfold incl, add in *. ss. des. split; ss.
+  - induction a0; ss. i. ss. des; subst; et.
+  - admit "siran".
 Qed.
 Next Obligation.
-  eapply Permutation.Permutation_NoDup; [|et].
-  eapply Permutation.Permutation_map.
-  eapply SkSort.sort_permutation.
+  unfold wf in *. des_ifs. ss. clarify. des. split.
+  - eapply Permutation.Permutation_NoDup; [|et].
+    eapply Permutation.Permutation_map.
+    apply Permutation.Permutation_app_comm.
+  - eapply Permutation.Permutation_NoDup; [|et].
+    eapply Permutation.Permutation_map.
+    admit "comm_perm".
 Qed.
 Next Obligation.
-  econs.
+  unfold wf in *. des_ifs. ss. clarify. des. split.
+  - eapply Permutation.Permutation_NoDup; [|et].
+    eapply Permutation.Permutation_map.
+    eapply SkGSort.sort_permutation.
+  - eapply Permutation.Permutation_NoDup; [|et].
+    eapply Permutation.Permutation_map.
+    eapply SkCSort.sort_permutation.
 Qed.
 Next Obligation.
-  cut (NoDup (map fst a)).
-  { i. eapply Permutation.Permutation_NoDup; [|et].
-      eapply Permutation.Permutation_map.
-      eapply SkSort.sort_permutation. }
-  cut (NoDup (map fst (a ++ b))).
-  { i. rewrite map_app in H0.
-      eapply nodup_app_l. et. }
-  i. eapply Permutation.Permutation_NoDup; [|et].
-  eapply Permutation.Permutation_map.
-  symmetry. eapply SkSort.sort_permutation.
+  split; econs.
+Qed.
+Next Obligation.
+  unfold wf in *. des_ifs. ss. clarify. des. split.
+  - cut (NoDup (map fst a)).
+    { i. eapply Permutation.Permutation_NoDup; [|et].
+        eapply Permutation.Permutation_map.
+        eapply SkGSort.sort_permutation. }
+    cut (NoDup (map fst (a ++ a0))).
+    { i. rewrite map_app in H1.
+        eapply nodup_app_l. et. }
+    i. eapply Permutation.Permutation_NoDup; [|et].
+    eapply Permutation.Permutation_map.
+    symmetry. eapply SkGSort.sort_permutation.
+  - cut (NoDup (map fst a2)).
+    { i. eapply Permutation.Permutation_NoDup; [|et].
+        eapply Permutation.Permutation_map.
+        eapply SkCSort.sort_permutation. }
+    (* cut (NoDup (map fst (a2 ++ a1))).
+    { i. rewrite map_app in H1.
+        eapply nodup_app_l. et. }
+    i. eapply Permutation.Permutation_NoDup; [|et].
+    eapply Permutation.Permutation_map.
+    symmetry. eapply SkCSort.sort_permutation. *)
+    admit "add no dup".
 Qed.
 
 Local Existing Instance gdefs.
 
 Definition load_skenv (sk: Sk.t): (SkEnv.t) :=
-  let n := List.length sk in
+  let n := List.length (fst sk) in
   {|
-      SkEnv.blk2id := fun blk => do '(gn, _) <- (List.nth_error sk blk); Some gn;
-      SkEnv.id2blk := fun id => do '(blk, _) <- find_idx (fun '(id', _) => string_dec id id') sk; Some blk
+      SkEnv.blk2id := fun blk => do '(gn, _) <- (List.nth_error (fst sk) blk); Some gn;
+      SkEnv.id2blk := fun id => do '(blk, _) <- find_idx (fun '(id', _) => string_dec id id') (fst sk); Some blk
   |}
   .
 
@@ -134,32 +298,32 @@ Lemma load_skenv_wf sk
     <<WF: SkEnv.wf (load_skenv sk)>>
 .
 Proof.
-  r in WF.
+  r in WF. ss. unfold wf in WF. des_ifs. des. 
   rr. split; i; ss.
   - uo; des_ifs.
-    + f_equal. ginduction sk; ss. i. inv WF.
+    + f_equal. ginduction a; ss. i. inv WF.
       rewrite find_idx_red in Heq1. des_ifs; ss.
       { destruct string_dec in Heq; clarify. }
       des_sumbool. uo. des_ifs. destruct p. ss.
-      hexploit IHsk; et.
-    + exfalso. ginduction sk; ss. i. inv WF.
+      hexploit IHa; et.
+    + exfalso. ginduction a; ss. i. inv WF.
       rewrite find_idx_red in Heq2. des_ifs; ss.
       des_sumbool. uo. des_ifs. destruct p. ss.
-      hexploit IHsk; et.
-  - ginduction sk; ss.
+      hexploit IHa; et.
+  - ginduction a; ss.
     { i. uo. ss. destruct blk; ss. }
     i. destruct a. inv WF. uo. destruct blk; ss; clarify.
     { rewrite find_idx_red. uo. des_ifs; destruct string_dec in *; ss. }
-    hexploit IHsk; et. i.
+    hexploit IHa; et. i.
     rewrite find_idx_red. uo. des_ifs; des_sumbool; ss. exfalso.
-    subst. clear - Heq1 H2. ginduction sk; ss. i.
+    subst. clear - Heq1 H2. ginduction a0; ss. i.
     rewrite find_idx_red in Heq1.
     des_ifs; destruct string_dec; ss; et.
-    uo. des_ifs. destruct p. eapply IHsk; et.
+    uo. des_ifs. destruct p. eapply IHa0; et.
 Qed.
 
 Definition incl_env (sk0: Sk.t) (skenv: SkEnv.t): Prop :=
-  forall gn gd (IN: List.In (gn, gd) sk0),
+  forall gn gd (IN: List.In (gn, gd) (fst sk0)),
   exists blk, <<FIND: skenv.(SkEnv.id2blk) gn = Some blk>>.
 
 Lemma incl_incl_env sk0 sk1
@@ -167,17 +331,18 @@ Lemma incl_incl_env sk0 sk1
 :
     incl_env sk0 (load_skenv sk1).
 Proof.
+  unfold incl in *. des.
   ii. exploit INCL; et. i. ss. uo. des_ifs; et.
-  exfalso. clear - x0 Heq0. ginduction sk1; et.
+  exfalso. clear - x0 Heq0. destruct sk1. ss. ginduction a; et.
   i. ss. rewrite find_idx_red in Heq0. des_ifs.
   des_sumbool. uo.  des_ifs. des; clarify.
-  eapply IHsk1; et.
+  eapply IHa; et.
 Qed.
 
 Lemma in_env_in_sk :
   forall sk blk symb
         (FIND: SkEnv.blk2id (load_skenv sk) blk = Some symb),
-  exists def, In (symb, def) sk.
+  exists def, In (symb, def) (fst sk).
 Proof.
   i. unfold SkEnv.blk2id. ss.
   uo. des_ifs. des; clarify.
@@ -186,37 +351,38 @@ Qed.
 
 Lemma in_sk_in_env :
   forall sk def symb
-        (IN: In (symb, def) sk),
+        (IN: In (symb, def) (fst sk)),
   exists blk, SkEnv.blk2id (load_skenv sk) blk = Some symb.
 Proof.
   i. unfold SkEnv.blk2id. ss.
   uo. eapply In_nth_error in IN. des.
-  eexists. rewrite IN. et.
+  exists n. unfold alist in *. rewrite IN. et.
 Qed.
 
 Lemma env_range_some :
   forall sk blk
-        (BLKRANGE : blk < Datatypes.length sk),
+        (BLKRANGE : blk < Datatypes.length (fst sk)),
   <<FOUND : exists symb, SkEnv.blk2id (load_skenv sk) blk = Some symb>>.
 Proof.
-  i. depgen sk. induction blk; i; ss; clarify.
-  - destruct sk; ss; clarify. { lia. }
+  i. destruct sk. ss. depgen l. induction blk; i; ss; clarify.
+  - destruct l; ss; clarify. { lia. }
     uo. destruct p. exists s. ss.
-  - destruct sk; ss; clarify. { lia. }
+  - destruct l; ss; clarify. { lia. }
     apply lt_S_n in BLKRANGE. eapply IHblk; eauto.
 Qed.
 
 Lemma env_found_range :
   forall sk symb blk
         (FOUND : SkEnv.id2blk (load_skenv sk) symb = Some blk),
-  <<BLKRANGE : blk < Datatypes.length sk>>.
+  <<BLKRANGE : blk < Datatypes.length (fst sk)>>.
 Proof.
-  induction sk; i; ss; clarify.
+  intros sk. destruct sk. ss.
+  induction a; i; ss; clarify.
   uo; des_ifs. destruct p0. rewrite find_idx_red in Heq0. des_ifs.
   { apply Nat.lt_0_succ. }
   destruct blk.
   { apply Nat.lt_0_succ. }
-  uo. des_ifs. destruct p. ss. clarify. apply lt_n_S. eapply IHsk; eauto.
+  uo. des_ifs. destruct p. ss. clarify. apply lt_n_S. eapply IHa; eauto.
   instantiate (1:=symb). rewrite Heq0. ss.
 Qed.
 
@@ -224,20 +390,20 @@ Lemma sk_incl_gd sk0 sk1 gn blk gd:
   Sk.wf sk1 ->
   Sk.le sk0 sk1 ->
   SkEnv.id2blk (load_skenv sk1) gn = Some blk ->
-  In (gn, gd) sk0 ->
-  nth_error sk1 blk = Some (gn, gd).
+  In (gn, gd) (fst sk0) ->
+  nth_error (fst sk1) blk = Some (gn, gd).
 Proof.
-  ss. i. red in H0. hexploit H0; et. i.
-  clear - H3 H1 H. ginduction sk1; i; ss.
+  ss. i. destruct sk0. destruct sk1. unfold incl in H0. ss. des. hexploit H0; et. i.
+  clear - H H1 H5. ginduction a1; i; ss.
   destruct blk; ss.
   - des; clarify. uo. des_ifs. rewrite find_idx_red in Heq0. exfalso.
     des_ifs; des_sumbool; subst.
-    + ss. inv H. eapply in_map with (f:=fst) in H3. et.
+    + ss. inv H. eapply in_map with (f:=fst) in H5. et.
     + uo. des_ifs.
   - des; clarify. uo. des_ifs. rewrite find_idx_red in Heq0.
     des_ifs; des_sumbool; subst.
     { exfalso. et. }
-    eapply IHsk1; et.
+    eapply IHa1; et.
     + inv H. et.
     + uo. rewrite find_idx_red in H1. des_ifs.
       uo. unfold curry2 in *. clarify.
