clightplus/proofmode/CIProofMode.v
@@ -878,7 +878,8 @@ Global Opaque equiv_prov.
 Global Opaque has_offset.
 Global Opaque points_to.
 Global Opaque ccallU.
-Global Opaque get_sk.
+Global Opaque get_ge.
+Global Opaque get_ce.
 Global Opaque build_composite_env'.
 Global Opaque build_composite_env.
 
